\documentclass[12pt]{article}
\usepackage{tikz}
\usepackage{harpoon}% <---
\usepackage{setspace}
\usepackage{extsizes}
\usepackage{float}
\usepackage{amsmath, amsthm, amssymb}    
\usepackage[margin=.5in]{geometry}


\title{\vspace{-2.0cm}Homework 7}
\author{Joanne Wardell}
\date{Thursday, September 20, 2018}
\begin{document}
\maketitle


\subsection*{Section 14.1}


\noindent 2.) $f(x, y) - \sin(xy)$\\
\noindent a.) $f(2, \frac{\pi}{6})$\\\\
\noindent b.) $f(-3, \frac{\pi}{12})$\\\\
\noindent c.) $f(\pi, \frac{1}{4})$\\\\
\noindent d.) $f(-\frac{\pi}{2}, -7)$\\\\

\noindent 6.) $f(x, y) = \ln{x^{2} + y^{2} - 4}$\\\\
\noindent 8.) $f(x, y) = \frac{\sin(xy)}{x^{2} + y^{2} - 25}$\\\\
\noindent 14.) $f(x,y) = x^{2} + y^{2}$, \hspace{10pt} $c = 0, 1, 4, 9, 16, 25$\\
\noindent Below is a sketch of the level curves.\vspace{4cm}\\\\
\noindent 32.) The level curves correspond to graph \textbf{b} and equation \textbf{i}.\\\\
\noindent 34.) The level curves correspond to graph \textbf{c} and equation \textbf{h}.\\\\
\noindent 36.) The level curves correspond to graph \textbf{e} and equation \textbf{j}.\\\\
\noindent 44.) $f(x, y) = \sqrt{x^{2} + y^{2}}$\\
\noindent a.) Below is a sketch of the surface.\vspace{4cm}
\noindent b.) Below is an assortment of level curves in the function's domain.\vspace{4cm}\\\\
\noindent 48.) $f(x, y) = \sqrt{x^{2} +y^{2} -4}$\\
\noindent a.) Below is a sketch of the surface.\vspace{4cm}\\\\
\noindent b.) Below is an assortment of level curves in the function's domain.\vspace{4cm}\\\\
\noindent 60.) $f(x, y, z) = \frac{x^{2}}{25} + \frac{y^{2}}{16} + \frac{z^{2}}{9}$\\
\noindent Below is a typical level surface for the function.\vspace{4cm}




\subsection*{Section 14.2}

\noindent 4.) $\lim\limits_{(x,y) \to (3,4)} \sqrt{x^{2} + y^{2} - 1}$\\\\
\noindent 16.) $\lim\limits_{(x,y) \to (2,2)} \frac{y+4}{x^{2}y -xy + 4x^{2} - 4x}$\\\\
\noindent 26.) $\lim\limits_{P \to (1, -1, -1)}\frac{2xy+yz}{x^{2}+z^{2}}$\\\\
\noindent 32.) \\
\noindent a.) $f(x, y) = \frac{x+y}{x-y}$\\\\
\noindent b.) $f(x,y) = \frac{y}{x^{2} + 1}$\\\\
\noindent 36.) \\
\noindent a.) $f(x, y,z) = \ln(xyz)$\\\\
\noindent b.) $f(x, y,z) = e^{x+y}\cos(z)$\\\\
\noindent 46.)$g(x,y) = \frac{x^{2}-y}{x -y}$\\\\


\end{document}
