\documentclass[12pt]{article}
\usepackage{setspace}
\usepackage{extsizes}
\usepackage{float}
\usepackage{amsmath, amsthm, amssymb}    
\usepackage[margin=.5in]{geometry}
\usepackage{tikz}
\usepackage{forest}


\title{\vspace{-2.0cm}Homework 8}
\author{Joanne Wardell}
\date{Tuesday, September 25, 2018}
\begin{document}
\maketitle
\subsection*{Section 14.3}
\noindent 4.) $f(x,y) = 5xy-7x^{2}-y^{2}+3x-6y+2$\\\\
\noindent $\frac{\partial f}{\partial x} =  14x + 8$\\\\
\noindent $\frac{\partial f}{\partial y} = 5x -2y -6$\\\\


\noindent 10.) $f(x,y) = \frac{x}{x^{2}+y^{2}}$\\\\
\noindent $\frac{\partial f}{\partial x} =  \frac{y^{2} - x^{2}}{(x^{2} + y^{2})^{2}}$\\\\
\noindent $\frac{\partial f}{\partial y} = \frac{x^{2} + y^{2} - 2xy}{(x^{2} + y^{2})^{2}}$\\\\

\noindent 16.) $f(x,y) = e^{xy}\ln{y}$\\\\
\noindent $\frac{\partial f}{\partial x} =  \frac{y^{2} - x^{2}}{(x^{2} + y^{2})^{2}}$\\\\
\noindent $\frac{\partial f}{\partial y} = \frac{x^{2} + y^{2} - 2xy}{(x^{2} + y^{2})^{2}}$\\\\


\noindent 24.) $f(x,y,z) = xy+yz+xz$\\\\
\noindent $f_{x} = \frac{\partial f}{\partial x} = y + z$\\\\
\noindent $f_{y} = \frac{\partial f}{\partial y} = x + z$\\\\
\noindent $f_{z} = \frac{\partial f}{\partial z} = y + x$\\\\


\noindent 26.) $f(x,y,z)=(x^{2}+y^{2}+z^{2})^{-\frac{1}{2}}$\\\\
\noindent $f_{x} = \frac{\partial f}{\partial x} = -x$\\\\
\noindent $f_{y} = \frac{\partial f}{\partial y} = -y$\\\\
\noindent $f_{z} = \frac{\partial f}{\partial z} = -z$\clearpage


\noindent 32.) $f(x,y,z) = e^{-xyz}$\\\\
\noindent $f_{x} = \frac{\partial f}{\partial x} = -yze^{-xyz}$\\\\
\noindent $f_{y} = \frac{\partial f}{\partial y} = -xze^{-xyz}$\\\\
\noindent $f_{z} = \frac{\partial f}{\partial z} = -xye^{-xyz}$\\\\



\noindent 38.) $g(r, \theta, z) = r(1-\cos{\theta}) - z$\\\\
\noindent $\frac{\partial g}{\partial r} = 1-\cos{\theta}$\\\\
\noindent $\frac{\partial g}{\partial \theta} = -r\sin{\theta}$\\\\
\noindent $\frac{\partial g}{\partial z} = -1$\\\\


\noindent 42.) $f(x,y)=\sin{xy}$\\\\
\noindent $\frac{\partial ^{2}f}{\partial x^{2}} = -y^{2}\sin{xy}$\\\\
\noindent $\frac{\partial ^{2} f}{\partial y^{2}} = -x^{2}\sin{xy}$\\\\
\noindent $\frac{\partial ^{2} f}{\partial x \partial y} = -xy\sin{xy} + \cos{xy}$\\\\
\noindent $\frac{\partial ^{2} f}{\partial y \partial x} = -xy\sin{xy} + \cos{xy}$\\\\



\noindent 58.) $w = x\sin{y} + y\sin{x} + xy$\\\\
\noindent $w_{xy} = \frac{\partial ^{2}w}{\partial y \partial x} = 1 + \cos{y} + \cos{x}$\\\\
\noindent $w_{yx} = \frac{\partial ^{2}w}{\partial x \partial y} = 1 + \cos{y} + \cos{x}$\\\\

\noindent 84.) $f(x,y,z)=2z^{3}-3(x^{2}+y^{2})z$\\\\
\noindent The \textbf{Laplace equation} is $\frac{\partial ^{2}f}{\partial x^{2}} + 
\frac{\partial ^{2}f}{\partial y^{2}} + \frac{\partial^{2} f}{\partial y^{2}} = 0$.\\\\
\noindent $\frac{\partial ^{2}f}{\partial x^{2}} = -6z$\\\\
\noindent $\frac{\partial ^{2}f}{\partial y^{2}} = -6z$\\\\
\noindent $\frac{\partial ^{2}f}{\partial z^{2}} = 12z$\\\\
\noindent $\frac{\partial ^{2}f}{\partial x^{2}} + \frac{\partial ^{2}f}{\partial y^{2}} + \frac{\partial^{2} f}{\partial y^{2}} = 
-6z -6z + 12z = 0$\\\\ 


\subsection*{Section 14.4}
\noindent 2.) $w = x^{2} + y^{2}$, \hspace{10pt} $x = \cos{t} + \sin{t}$, \hspace{10pt} $y = \cos{t} - \sin{t}$, \hspace{10pt} $t=0$\\\\
\noindent $\frac{dw}{dt} = \frac{\partial w}{\partial x} \frac{dx}{dt} + \frac{\partial w}{\partial y}\frac{dy}{dt}
=\frac{\partial (x^{2} + y^{2})}{\partial x}\frac{d(\cos{t} + \sin{t})}{dt} 
+ \frac{\partial (x^{2} + y^{2})}{\partial y}\frac{d(\cos{t}\sin{t})}{dt} = 2\cos^{t}-2\sin^{2}{t}-2\cos^{2}{t}+2\sin^{2}{t} = 0$\\\\



\noindent 10.) $w = \ln(x^{2}+y^{2} + z^{2})$, \hspace{10pt} $x = ue^{v}\sin{u}$, 
\hspace{10pt} $y = ue^{v}\cos{u}$, \hspace{10pt} $z = ue^{v}$; \hspace{10pt} $(u,v) = (-2,0)$\\\\
\noindent $\frac{\partial w}{\partial u} = \frac{\partial w}{\partial x}\frac{\partial x}{\partial u} 
+\frac{\partial w}{\partial y}\frac{\partial y}{\partial u}+ \frac{\partial w}{\partial z}\frac{\partial z}{\partial u}$\\\\
\noindent $\frac{\partial w}{\partial x} = \frac{2x}{x^{2} + y^{2} + z^{2}}$\\\\
\noindent $\frac{\partial x}{\partial u} = e^{v}\sin{u} + e^{v}u\cos{u}$\\\\
\noindent $\frac{\partial w}{\partial y} = \frac{2y}{x^{2} + y^{2} +z^{2}}$\\\\
\noindent $\frac{\partial y}{\partial u} = e^{v}\cos{u} - e^{v}u\sin{u}$\\\\
\noindent $\frac{\partial w}{\partial z} = \frac{2z}{x^{2} + y^{2} + z^{2}}$\\\\
\noindent $\frac{\partial z}{\partial u} = e^{v}$\\\\
\noindent $\frac{\partial w}{\partial u} =[e^{v}\sin{u}+e^{v}u\cos{u}]\frac{2x}{x^{2} + y^{2} +z^{2}} 
+ [e^{v}\cos{u}-e^{v}u\sin{u}]\frac{2y}{x^{2} + y^{2} + z^{2}} + [e^{v}]\frac{2z}{x^{2} + y^{2} + z^{2}}
\\\\ =  [e^{v}\sin{u}+e^{v}u\cos{u}]\frac{2ue^{v}\sin{u}}{u^{2}e^{2v}\sin^{2}{u}+u^{2}e^{2v}\cos^{2}{u}+u^{2}e^{2v}} 
\\\\+ [e^{v}cos{u}-ue^{v}u\sin{u}]\frac{2ue^{v}\cos{u}}{u^{2}e^{2v}\sin^{2}{u}+u^{2}e^{2v}\cos^{2}{u}+u^{2}e^{2v}} 
\\\\+ [e^{2v}]\frac{2ue^{v}}{u^{2}e^{2v}\sin^{2}{u}+u^{2}e^{2v}\cos^{2}{u}+u^{2}e^{2v}} 
= \frac{2}{u}$\\\\




\noindent $\frac{\partial w}{\partial v} = \frac{\partial w}{\partial x}\frac{\partial x}{\partial v} 
+\frac{\partial w}{\partial y}\frac{\partial y}{\partial v}+ \frac{\partial w}{\partial z}\frac{\partial z}{\partial v}$\\\\
\noindent $\frac{\partial w}{\partial x} = \frac{2x}{x^{2} + y^{2} + z^{2}}$\\\\
\noindent $\frac{\partial x}{\partial v} = e^{v}u\sin{u}$\\\\
\noindent $\frac{\partial w}{\partial y} = \frac{2y}{x^{2} + y^{2} +z^{2}}$\\\\
\noindent $\frac{\partial y}{\partial v} = ue^{v}\cos{u}$\\\\
\noindent $\frac{\partial w}{\partial z} = \frac{2z}{x^{2} + y^{2} + z^{2}}$\\\\
\noindent $\frac{\partial z}{\partial v} = e^{v}u$\\\\
\noindent $\frac{\partial w}{\partial v} =[u^{2}e^{v}\cos{u}]\frac{2x}{x^{2} + y^{2} +z^{2}} 
+ [u^{2}e^{v}\cos{u}]\frac{2y}{x^{2} + y^{2} + z^{2}} + [e^{v}u^{2}]\frac{2z}{x^{2} + y^{2} + z^{2}}
\\\\ =  [u^{2}e^{v}\cos{u}]\frac{2ue^{v}\sin{u}}{u^{2}e^{2v}\sin^{2}{u}+u^{2}e^{2v}\cos^{2}{u}+u^{2}e^{2v}} 
\\\\+ [u^{2}e^{v}\cos{u}]\frac{2ue^{v}\cos{u}}{u^{2}e^{2v}\sin^{2}{u}+u^{2}e^{2v}\cos^{2}{u}+u^{2}e^{2v}} 
\\\\+ [e^{v}u^{2}]\frac{2ue^{v}}{u^{2}e^{2v}\sin^{2}{u}+u^{2}e^{2v}\cos^{2}{u}+u^{2}e^{2v}} 
$\\\\


\noindent $w = \ln(x^{2} + y^{2} + z^{2})= \ln[(ue^{v}\sin{u})^{2} + (ue^{v}\cos{u})^{2} + (ue^{v})^{2}]
\\=\ln(u^{2}e^{2v}\sin^{2}{u} + u^{2}e^{2v}\cos^{2}{u} + u^{2}e^{2v})
\\= \ln(u^{2}e^{2v}(\sin^{2}{u} + \cos^{2}{u}) + u^{2}e^{2v})
\\=\ln(2u^{2}e^{2v}) = \ln{2} + 2\ln{u} + 2v\ln{e} = \ln{2} + 2\ln{u}$\\\\

\noindent $\frac{\partial w}{\partial u} = \frac{\partial (\ln{2} + 2\ln{u} + 2v)}{\partial u} = \frac{2}{u}$\\\\

\noindent $\frac{\partial w}{\partial v} = \frac{\partial (\ln{2} + 2\ln{u} + 2v)}{\partial v} = 2$\\\\


\noindent 16.) $\frac{\partial w}{\partial x}$ and $\frac{\partial w}{\partial y}$ for $w = f(r,s,t)$,
 \hspace{10pt} $r = g(x,y)$, \hspace{10pt} $s = h(x,y)$, \hspace{10pt} $t = k(x,y)$\\\\

\noindent $\frac{\partial w}{\partial x} = \frac{\partial w}{\partial r}\frac{\partial r}{\partial x} 
+ \frac{\partial w}{\partial s}\frac{\partial s}{\partial x} + \frac{\partial w}{\partial t}\frac{\partial t}{\partial x}$ \\\\
\vspace{6cm}\\\\



%\begin{forest}
%[$w$[$r$][$s$’[$x$]][$t$’[$x$]]]
%\end{forest}
%dont have time for tree even tho i really want to do it >:[

\noindent $\frac{\partial w}{\partial y} = \frac{\partial w}{\partial r}\frac{\partial r}{\partial y} 
+ \frac{\partial w}{\partial s}\frac{\partial s}{\partial y} + \frac{\partial w}{\partial t}\frac{\partial t}{\partial y}$ \\\\
\vspace{6cm}\\\\



\noindent 22.) $\frac{\partial w}{\partial p}$ for $w = f(x,y,z,v)$, \hspace{10pt} $x = g(p,q)$, 
\hspace{10pt} $y = h(q,p)$, \hspace{10pt} $z = j(p,q)$, \hspace{10pt} $v = k(p,q)$\\\\
\noindent $\frac{\partial w}{\partial p} = \frac{\partial w}{\partial x}\frac{\partial x}{\partial p} 
+ \frac{\partial w}{\partial y}\frac{\partial y}{\partial p} + \frac{\partial w}{\partial z}\frac{\partial z}{\partial p} +
 \frac{\partial w}{\partial v}\frac{\partial v}{\partial p}$\\\\
\vspace{6cm}\\\\


\noindent 34.) $xe^{y} + ye^{z} + 2\ln{x}-2 -3\ln{2} = 0$, \hspace{10pt} $(1, \ln{2}, \ln{3})$\\\\
\noindent $f_{x} = \frac{\partial f}{\partial x} = e^{y}+\frac{2}{x}$\\\\
\noindent $f_{y} = \frac{\partial f}{\partial y} = xe^{y}+e^{z}$\\\\
\noindent $f_{z} = \frac{\partial f}{\partial z} = ye^{z}$\\\\
\noindent $\frac{\partial z}{\partial x} = -\frac{f_{x}}{f_{z}} = \frac{e^{y}+\frac{2}{x}}{ye^{z}}$
\noindent $\frac{e^{y}+\frac{2}{x}}{ye^{z}}\Big|_{1, \ln{2}, \ln{3}} = -\frac{4}{3\ln{2}}$\\\\
\noindent $\frac{\partial z}{\partial y} = -\frac{f_{y}}{f_{z}} = -\frac{xe^{y}+e^{z}}{ye^{z}}$
\noindent $-\frac{f_{y}}{f_{z}} = -\frac{xe^{y}+e^{z}}{ye^{z}}\Big|_{1, \ln{2}, \ln{3}} = -\frac{5}{3\ln{2}}$\\\\

\noindent 38.)  \hspace{10pt}$z = \sin{xy} + x\sin{y}$, \hspace{10pt} $x = u^{2} 
+ v^{2}$, \hspace{10pt} $y = uv$, \hspace{10pt} $\frac{\partial z}{\partial u} \Big|_{u = 0, v=1}$\\\\
\noindent $\frac{\partial z}{\partial u} = \frac{\partial z}{\partial x}\frac{\partial x}{u} 
+ \frac{\partial z}{\partial y}\frac{\partial y}{\partial u}$\\\\
\noindent $\frac{\partial z}{\partial x} = y\cos{xy} + \sin{y}$\\\\
\noindent $\frac{\partial z}{\partial y} = x\cos{xy} + x\cos{y}$\\\\
\noindent $\frac{\partial x}{\partial u} = 2u$\\\\
\noindent $\frac{\partial y}{\partial u} = v$\\\\

\noindent $\frac{\partial z}{\partial u} = 2uy\cos{xy} + 2u\sin{y} + vx\cos{xy} + xv\cos{y}
\\\\= [vu\cos(u^{3}v + uv^{3}) + \sin{uv}]2u + [(u^{2}+v^{2})\cos{(u^{3}v + uv^{3}) + (u^{2} + v^{2})\cos{uv}}]v$\\\\


\noindent $\frac{\partial z}{\partial u} \Big|_{u = 0, v=1} = 0+\cos{0} + \cos{0} = 2$\\\\



\noindent 50.) $w = f(x,y)$, \hspace{10pt} $x = r\cos{\theta}$, \hspace{10pt} $y = r\sin{\theta}$\\\\
\noindent $x_{r} = \frac{\partial r\cos{\theta}}{\partial r} = \cos{\theta}$\\\\
\noindent $y_{r} = \frac{\partial r\sin{\theta}}{\partial r} = \sin{\theta}$\\\\
\noindent a.) $\frac{\partial w}{\partial r} = \frac{\partial w}{\partial x}\frac{\partial x}{r}
 + \frac{\partial w}{\partial y}\frac{\partial y}{\partial r} = x_{r}\frac{\partial f}{\partial x} 
+ y_{r}\frac{\partial f}{\partial y} = \cos{\theta}\frac{\partial f}{\partial x} + \sin{\theta}\frac{\partial f}{\partial y}$
\\\\$\frac{\partial f}{\partial \theta} = \frac{\partial f}{\partial x}\frac{\partial x}{\partial \theta} 
+ \frac{\partial f}{\partial y}\frac{\partial y}{\partial \theta} 
= -rf_{x}\sin{\theta} + rf_{y}\cos{\theta} = r[f_{y}\cos{\theta} - f_{x}\sin{\theta}]$\\\\
\noindent $\therefore \frac{1}{r}\frac{\partial w}{\partial \theta} = f_{y}\cos{\theta} - f_{x}\sin{\theta}$\\\\
\noindent b.)$f_{x} = (\cos{\theta})\frac{\partial w}{\partial r}-(\frac{\sin{\theta}}{r})\frac{\partial w}{\partial \theta}$\\\\
$f_{y} = (\sin{\theta})\frac{\partial w}{\partial r} + (\frac{\cos{\theta}}{r})\frac{\partial w}{\partial \theta}$\\\\

\noindent c.) $(f_{x})^{2} + (f_{y})^{2} = (\frac{\partial w}{\partial r})^{2} +
 \frac{1}{r^{2}}(\frac{\partial w}{\partial \theta})^{2}$\\\\
\noindent $(f_{x})^{2} = (\cos^{2}{\theta})(\frac{\partial w}{\partial r})^{2} +
 (\frac{\sin^{2}{\theta}}{r^{2}})(\frac{\partial w}{\partial \theta})^{2} - 
2(\cos{\theta}\frac{\partial w}{\partial r}\frac{\sin{\theta}}{r}\frac{\partial w}{\partial \theta})$\\\\
\noindent $(f_{y})^{2} = (\sin^{2}{\theta})(\frac{\partial w}{\partial r})^{2} +
 (\frac{\cos^{2}{\theta}}{r^{2}})(\frac{\partial w}{\partial \theta})^{2} + 
2(\sin{\theta}\frac{\partial w}{\partial r}\frac{\cos{\theta}}{r}\frac{\partial w}{\partial \theta})$\\\\
\noindent $\therefore (f_{x})^{2} + (f_{y})^{2} = (\frac{\partial w}{\partial r})^{2} + 
\frac{1}{r^{2}}(\frac{\partial w}{\partial \theta})^{2}$\\\\ 


\end{document}
