\documentclass[12pt]{article}
\usepackage{setspace}
\usepackage{extsizes}
\usepackage{float}
\usepackage{amsmath, amsthm, amssymb}    
\usepackage[margin=.5in]{geometry}
\usepackage{tikz}
\usepackage{forest}


\title{\vspace{-2.0cm}Homework 8}
\author{Joanne Wardell}
\date{Tuesday, September 25, 2018}
\begin{document}
\maketitle

\subsection*{Section 14.5}

\noindent 4.) $g(x,y) = \frac{x^{2}}{2} -\frac{y^{2}}{2}$, \hspace{10pt} $(\sqrt{2},1)$\\\\
\noindent $\nabla f \Big|_{(2,1)} = \langle \frac{\partial g}{\partial x}, \frac{\partial g}{\partial y} \rangle \Big|_{(\sqrt{2}, 1)}
= \langle \sqrt{2}, -1\rangle$\\\\
\noindent $g(\sqrt{2}, 1) = \frac{1}{2}$\\\\
\noindent $\frac{1}{2} = \frac{x^{2}}{2} - \frac{y^{2}}{2}$\\\\
\noindent The level curve is $1 = x^{2} - y^{2}$
\noindent 8.) $f(x, y, z) = 2z^{3} - 3(x^{2} + y^{2})z \arctan{xz}$, \hspace{10pt} $(1,1,1)$\\\\
\noindent $\nabla f \Big|_{(1,1,1)} = \langle \frac{\partial f}{\partial x}, \frac{\partial f}{\partial y}, \frac{\partial f}{\partial z} \rangle \Big|_{(1,1,1)}$\\\\
\noindent $\frac{\partial f}{\partial x} = 2x + \frac{z}{x}$\\\\
\noindent $\frac{\partial f}{\partial x}\Big|_{(1, 1, 1)} = 3$\\\\

\noindent $\frac{\partial f}{\partial y} = 2y$\\\\
\noindent $\frac{\partial f}{\partial y}\Big|_{(1, 1, 1)} = 2$\\\\

\noindent $\frac{\partial f}{\partial z} = -4z+\ln{x}$\\\\
\noindent $\frac{\partial f}{\partial z}\Big|_{(1, 1, 1)} = -4$\\\\

\noindent 12.) $f(x,y) = 2x^{2} + y^{2}$, \hspace{10pt} $p_{0}(-1,1)$, \hspace{10pt} $\mathbf{u} = 4\mathbf{i} + 3\mathbf{j}$\\\\
\noindent $\hat{u} = \frac{\mathbf{u}}{\| \mathbf{u} \|} = \frac{1}{5} \langle 4, 3\rangle$\\\\
\noindent $f_{x} = 4x$, \hspace{10pt} $f_{y} = 2y$\\
\noindent $\nabla f \Big|_{(-1, 1)} = \langle -4, 2\rangle$\\\\
\noindent $\nabla f \frac{\mathbf{u}}\cdot {\| \mathbf{u} \|} = \langle -4, 2\rangle \cdot \langle \frac{3}{5} , \frac{4}{5}\rangle = -4$\\\\
\noindent 16.) $f(x, y, z) = x^{2} + 2y^{2} - 3z^{2}$, \hspace{10pt} $\mathbf{u} = \mathbf{i} + \mathbf{j} + \mathbf{k}$, \hspace{10pt} $P_{0}(1, -1, 2)$\\\\
\noindent $f_{x} \Big|_{(1, 1, 1)} = 2x \Big|{(1, 1, 1)} = 2$\\
\noindent $f_{y} \Big|_{(1, 1, 1)} = 4y \Big|{(1, 1, 1)} = 4$\\
\noindent $f_{z} \Big|_{(1, 1, 1)} = -6z \Big|{(1, 1, 1)} = -6$\\\\
\noindent $\hat{u} =\frac{\mathbf{u}} {\| \mathbf{u} \| } = \frac{1}{\sqrt{3}} \langle 1, 1, 1 \rangle$\\\\
\noindent $D_{u}f = \nabla f \cdot \frac{\mathbf{u}}{\| \mathbf{u} \|} = \langle 2, 4, -6\rangle \cdot \langle\frac{1}{\sqrt{3}}, \frac{1}{\sqrt{3}}, \frac{1}{\sqrt{3}} \rangle = 0$\\\\
\noindent 22.) $g(x,y,z) = xe^{y} + z^{2}$, \hspace{10pt} $P_{0}(1,\ln{2}, \frac{1}{2})$\\\\
\noindent $\nabla g \Big|_{(1, \ln{2}, \frac{1}{2})} = \langle e^{y}, xe^{y}, 2z \rangle \Big|_{(1, \ln{2}, \frac{1}{2})} = \langle 2, 2, 1\rangle$\\\\
\noindent $\mathbf{u} = \frac{\nabla g}{\| \nabla g \|} = \langle \frac{2}{3}, \frac{2}{3}, \frac{2}{3}\rangle$\\\\
\noindent $D_{u}g\Big|_{P_{0}} = \nabla g \cdot \mathbf{u} = 3$\\
\noindent $D_{-u}g\Big|_{P_{0}} = \nabla g \cdot -\mathbf{u} = -3$\\\\
\noindent 28.) $x^{2} -xy + y^{2} = 7$, \hspace{10pt} $(-1, 2)$ \\\\
\noindent $f_{x} = 2x - y$\\
\noindent $f_{y} = -x + 2y$\\\\
\noindent $\nabla f \Big|_{(-1, 2)} = \langle 2x-y, -x+2y\rangle \Big|_{(-1, 2)} = \langle -4, 5\rangle$ \\\\
\noindent $f_{x}(x_{0}, y_{0})(x-x_{0}) + f_{y}(x_{0}, y_{0})(y-y_{0}) = -4x + 5y - 14$\\\\



\subsection*{Section 14.6}

\noindent 2.) $x^{2} + y^{2} - z^{2} = 18$, \hspace{10pt} $P_{0}(3, 5, -4)$\\\\
\noindent a.) $\nabla F \Big|_{(3, 5, -4)}= \langle 2,2, -2\rangle \Big|_{(3, 5, -4)} = \langle 6, 10, 8\rangle$\\\\
\noindent $f_{x}(x_{0}, y_{0}, z_{0})(x-x_{0}) + f_{y}(x_{0}, y_{0}, z_{0})(y-y_{0}) f_{z}(x_{0}, y_{0}, z_{0})(z - z_{0})= 3x + 5y + 4z = 18$\\\\
\noindent b.) The line normal to the surface at $P_{0}$ is $x = 3 + 6t$, \hspace{10pt} $y = 5 + 10t$, \hspace{10pt} $z = -4 + 8t$\\\\
\noindent 10.)$ye^{x} -ze^{y^{2}} = z$, \hspace{10pt} $P_{0}(0, 0, 1)$\\\\
\noindent a.) $\nabla f \Big|_{P_{0}} = \langle ye^{x}, e^{x} - 2yze^{y^{2}} \rangle \Big|_{P_{0}} = \langle0, 1 \rangle$\\\\
\noindent b.) The line normal to the surface at $P_{0}$ is $x = 0$, \hspace{10pt} $y = 0$, \hspace{10pt} $z = -1$\\\\
\noindent 12.) $z = e^{-(x^{2} + y^{2})}$, \hspace{10pt} $(0, 0, 1)$\\\\
\noindent $F_{x} (x, y) = -2xe^{-(x^{2} + y^{2})}$\\
\noindent $F_{y} (x, y) = -2ye^{-(x^{2} + y^{2})}$\\
\noindent $F_{x}(0,0) = 0$\\
\noindent $F_{y}(0,0) = 0$\\\\
\noindent The tangent plane at $(0,0,1)$ is $0(x-0) + 0(y-y) - (z -1) \leftarrow z = 1$\\\\
\noindent 22.) $\nabla f \Big|_{P_{0}} = \langle e^{x}\cos{yz}, ze^{x}\sin{yz}, -ye^{x}\sin{yz} \rangle \Big|_{P_{0}} = \langle 1, 0, 0\rangle$\\\\
\noindent $\nabla f \Big|_{P_{0}} \cdot \mathbf{u} = \langle 1, 0, 0\rangle \cdot \langle \frac{1}{\sqrt{3}}, \frac{1}{\sqrt{3}}, \frac{1}{\sqrt{3}}\rangle  = \frac{1}{sqrt{3}}$ \\\\


$df  = (\nabla f\Big|_{P_{0}} \cdot \mathbf{u})ds = \frac{1}{\sqrt{3}}(0.1) \approx 0.0577$\\\\
\noindent 32.) $$\\\\
\noindent 42.)


\end{document}
